Handle tReflect at the level of untyped syntax.

theories/Computation.v
@@ -47,6 +47,50 @@ Fixpoint qNat (n : nat) := match n with
 | S n => tSucc (qNat n)
 end.
 
+Fixpoint uNat (n : term) := match n with
+| tZero => Some 0
+| tSucc n =>
+  match uNat n with
+  | None => None
+  | Some n => Some (S n)
+  end
+| _ => None
+end.
+
+(* Builds the type [0 = 0 × ... × 0 = 0 × tSucc v = tSucc v] *)
+Fixpoint qEvalTy (n : nat) (v : nat) := match n with
+| 0 => tId tNat (tSucc (qNat v)) (tSucc (qNat v))
+| S n => tAnd (tId tNat tZero tZero) (qEvalTy n v)
+end.
+
+(* Builds a canonical proof of [0 = 0 × ... × 0 = 0 × tSucc v = tSucc v] *)
+Fixpoint qEvalTm (n : nat) (v : nat) := match n with
+| 0 => tRefl tNat (tSucc (qNat v))
+| S n => tPair (tId tNat tZero tZero) (qEvalTy n v) (tRefl tNat tZero) (qEvalTm n v)
+end.
+
+Lemma uNat_qNat : forall n, uNat (qNat n) = Some n.
+Proof.
+induction n; cbn; try congruence.
+rewrite IHn; eauto.
+Qed.
+
+Lemma qNat_uNat : forall t n, uNat t = Some n -> t = qNat n.
+Proof.
+intros t n; revert t; induction n; intros; destruct t; cbn in *; try discriminate.
++ reflexivity.
++ destruct (uNat t); cbn in *; discriminate.
++ remember (uNat t) as m eqn:Hm; symmetry in Hm; destruct m; cbn in *.
+  - f_equal; apply IHn; congruence.
+  - discriminate.
+Qed.
+
+Lemma qNat_inj : forall m n, qNat m = qNat n -> m = n.
+Proof.
+induction m; intros []; cbn; intros; try congruence.
+f_equal; apply IHm; congruence.
+Qed.
+
 Lemma qNat_ren : forall n ρ, (qNat n)⟨ρ⟩ = qNat n.
 Proof.
 intros n ρ; induction n; cbn in *; try f_equal; eauto.
@@ -60,6 +104,50 @@ Qed.
 Lemma closedn_qNat : forall n k, closedn k (qNat n).
 Proof.
 unfold closedn; induction n; intros; cbn in *; eauto.
+Qed.
+
+Lemma qEvalTy_ren : forall n v ρ, (qEvalTy n v)⟨ρ⟩ = qEvalTy n v.
+Proof.
+intros n; induction n; intros v ρ; cbn in *.
++ now rewrite qNat_ren.
++ unfold tAnd; f_equal.
+  rewrite !IHn; reflexivity.
+Qed.
+
+Lemma qEvalTy_subst : forall n v σ, (qEvalTy n v)[σ] = qEvalTy n v.
+Proof.
+intros n; induction n; intros v σ; cbn in *.
++ now rewrite qNat_subst.
++ unfold tAnd; f_equal.
+  rewrite qEvalTy_ren, !IHn; reflexivity.
+Qed.
+
+Lemma closedn_qEvalTy : forall n v k, closedn k (qEvalTy n v).
+Proof.
+unfold closedn; induction n; intros; cbn in *.
+- apply andb_true_intro; split; apply closedn_qNat.
+- apply closedn_shift, IHn.
+Qed.
+
+Lemma qEvalTm_ren : forall n v ρ, (qEvalTm n v)⟨ρ⟩ = qEvalTm n v.
+Proof.
+intros n; induction n; intros v ρ; cbn in *.
++ now rewrite qNat_ren.
++ rewrite !IHn, qEvalTy_ren; reflexivity.
+Qed.
+
+Lemma qEvalTm_subst : forall n v σ, (qEvalTm n v)[σ] = qEvalTm n v.
+Proof.
+intros n; induction n; intros v σ; cbn in *.
++ now rewrite qNat_subst.
++ rewrite !IHn, qEvalTy_subst; reflexivity.
+Qed.
+
+Lemma closedn_qEvalTm : forall n v k, closedn k (qEvalTm n v).
+Proof.
+unfold closedn; induction n; intros; cbn in *.
+- apply closedn_qNat.
+- apply IHn.
 Qed.
 
 (** Axiomatic definition of a computation model internal to MLTT *)
